vale/code/arch/x64/interop/GCMencryptOpt_stdcalls.fsti
@@ -18,6 +18,7 @@ open GHash_s
 open GCTR_s
 open GCTR
 open Interop.Base
+open Arch.Types
 
 let uint8_p = B.buffer UInt8.t
 let uint64 = UInt64.t
@@ -108,30 +109,19 @@ val gcm128_encrypt_opt_stdcall:
       (let db = get_downview keys_b in
       length_aux keys_b;
       let ub = UV.mk_buffer db Views.up_view128 in
-      Seq.equal (UV.as_seq h0 ub) (key_to_round_keys_LE AES_128 (Ghost.reveal key)))
+      Seq.equal (UV.as_seq h0 ub) (key_to_round_keys_LE AES_128 (Ghost.reveal key))) /\
+      le_bytes_to_quad32 (seq_uint8_to_seq_nat8 (Seq.slice (B.as_seq h0 hkeys_b) 0 16)) == 
+        aes_encrypt_LE AES_128 (Ghost.reveal key) (Mkfour 0 0 0 0)      
     )
     (ensures fun h0 _ h1 ->
       B.modifies (B.loc_union (B.loc_buffer tag_b)
                  (B.loc_union (B.loc_buffer iv_b)
                  (B.loc_buffer out_b))) h0 h1 /\
 
-      (let iv_LE = le_bytes_to_quad32 (seq_uint8_to_seq_nat8 (B.as_seq h0 iv_b)) in
-       let iv_BE = reverse_bytes_quad32 iv_LE in
-       let ctr_BE_1 = Mkfour 1 iv_BE.lo1 iv_BE.hi2 iv_BE.hi3 in
-       let ctr_BE_2 = Mkfour 2 iv_BE.lo1 iv_BE.hi2 iv_BE.hi3 in
-
-       let plain_in = le_bytes_to_seq_quad32 (pad_to_128_bits (seq_uint8_to_seq_nat8 (B.as_seq h0 plain_b))) in
-       let cipher_out = le_bytes_to_seq_quad32 (pad_to_128_bits (seq_uint8_to_seq_nat8 (B.as_seq h1 out_b))) in
-
-       DV.length_eq (get_downview hkeys_b);
-       length_aux5 hkeys_b;
-       let h = reverse_bytes_quad32 (low_buffer_read TUInt8 TUInt128 h1 hkeys_b 0) in
-       let length_quad = reverse_bytes_quad32 (Mkfour (8 * UInt64.v plain_len) 0 (8 * UInt64.v auth_len) 0) in
-      let auth_pad = le_bytes_to_seq_quad32 (pad_to_128_bits (seq_uint8_to_seq_nat8 (B.as_seq h0 auth_b))) in
-      let auth_in = Seq.append auth_pad (Seq.append cipher_out (Seq.create 1 length_quad)) in       
-
-      DV.length_eq (get_downview tag_b);
-      low_buffer_read TUInt8 TUInt128 h1 tag_b 0 ==
-         gctr_encrypt_block ctr_BE_1 (ghash_LE h auth_in) AES_128 (Ghost.reveal key) 0 /\
-      gctr_partial AES_128 (B.length plain_b / 16 + 1) plain_in cipher_out (Ghost.reveal key) ctr_BE_2)
+      (let iv = seq_uint8_to_seq_nat8 (B.as_seq h0 iv_b) in
+       let plain = seq_uint8_to_seq_nat8 (B.as_seq h0 plain_b) in
+       let auth = seq_uint8_to_seq_nat8 (B.as_seq h0 auth_b) in
+       let cipher, tag = gcm_encrypt_LE AES_128 (seq_nat32_to_seq_nat8_LE (Ghost.reveal key)) iv plain auth in
+       Seq.equal (seq_uint8_to_seq_nat8 (B.as_seq h1 out_b)) cipher /\
+       Seq.equal (seq_uint8_to_seq_nat8 (B.as_seq h1 tag_b)) tag)
   )
